coq-osiris/theories/proofmode/pure_tactics.v
@@ -1,0 +1,501 @@
+From osiris Require Import base.
+From osiris.lang Require Import lang.
+From osiris.semantics Require Import semantics.
+From osiris.proofmode Require Import simp_tactics pure_hoare simp_eval.
+From Ltac2 Require Ltac2.
+
+(* This file contains tactics intended for use during hoare-style proofs of pure
+   programs. These range from symbolic execution to tactics designed to aid
+   the application of single lemmas. *)
+
+(* -------------------------------------------------------------------------- *)
+
+(* Tactics. *)
+
+(* TODO reduce just beta-redexes in the goal (possibly under ∀ and →) *)
+
+Ltac beta :=
+  cbn beta.
+
+Goal (forall l : list nat,
+         l = [] ->
+         (λ (x : bool), negb x = ((λ (x : bool), x) false)) true).
+Proof.
+  beta. reflexivity.
+Qed.
+
+(* [remove_deco] is used by subsequent tactics when we want to match on an
+   expression under a decoration in a goal. *)
+
+Ltac remove_deco :=
+  lazymatch goal with
+  | |- pure (eval _ (deco _ _)) _ => unfold deco at 1; simpl
+  | _ => idtac
+  end.
+
+(* Remove any local environment definitions. *)
+
+Ltac clear_abstracted_env :=
+  repeat (match goal with
+          | η := _ : list (var * val) |- _ => subst η
+          end).
+
+(* [abstract_env] expects a goal of the form [pure (eval η e) φ]. It creates a
+   local definition for the environment [η]. *)
+
+Ltac abstract_env :=
+  lazymatch goal with
+  | |- pure (eval ?η _) _ =>
+      clear_abstracted_env;
+      match goal with
+      | |- pure (eval ?η _) _ =>
+          let η0 := fresh "η" in
+          set η as η0
+      end
+  | _ => idtac
+  end.
+
+Ltac extend_env :=
+  match goal with
+  | |- forall (η : env), η = _ -> _ =>
+      intros ? ->
+  | _ => idtac
+  end.
+
+(* -------------------------------------------------------------------------- *)
+
+(* [pure_ret] expects a goal of the form [pure (ret v) φ]. It applies
+   the lemma [pure_ret], solves the subgoal [v = #x], and leaves just
+   the subgoal [φ x], which it simplifies. *)
+
+Ltac pure_ret :=
+  remove_deco;
+  match goal with
+  | |- pure (ret ?v) ?φ =>
+      match type of φ with
+      | val -> Prop =>
+          simple eapply pure_ret; [ rewrite <- solve_encode_val; reflexivity | beta]
+      | _ =>
+          simple eapply pure_ret; [ solve [ encode ] | beta ]
+      end
+  end.
+
+(* [pure_path] expects a goal of the form [pure (eval η (EPath x)) φ]. It applies
+   the lemma [pure_eval_path], asks Coq to compute the lookup in the environment,
+   and, assuming that the lookup succeeds, calls pure_ret on the result. *)
+
+Ltac pure_path :=
+  remove_deco;
+  eapply pure_eval_path; simpl lookup_path;
+  match goal with
+  | H : lookup_name ?η ?path = ret ?res |- pure (lookup_name ?η ?path) _ =>
+      rewrite H
+  | _ => idtac
+  end;
+  pure_ret.
+
+(* [pure_const] expects a goal of the form [pure (eval η (EConstant x)) φ].
+   It applies the lemma [pure_eval_const], solves the subgoal [VConstant c = #x],
+   and leaves the subgoal [φ x]. *)
+
+Ltac pure_const :=
+  remove_deco;
+  match goal with
+  | |- pure (eval ?η (EConstant ?c)) ?ψ =>
+      match type of ψ with
+      | val -> Prop =>
+          simple eapply pure_eval_const; [ rewrite <- solve_encode_val; reflexivity | ]
+      | _ =>
+          simple eapply pure_eval_const; [ solve [ encode ] | ]
+      end
+  end.
+
+Local Open Scope nat.
+
+Ltac pure_data :=
+  remove_deco;
+  simpl;
+  match goal with
+  | |- pure (eval _ (EData ?c (ETuple ?args))) _ =>
+      match eval cbn in (length args) with
+      | 0 => pure_const
+      | 1 => eapply pure_eval_data1
+      | 2 => eapply pure_eval_data2; eapply pure_eval_pair
+      | 3 => eapply pure_eval_data3; eapply pure_eval_triple
+      | 4 => eapply pure_eval_data4
+      (* TODO: make a higher-order version of pure_eval_pair *)
+      | _ => fail "Not implemented for this arity"
+      end
+  end;
+  repeat (pure_path || pure_const || pure_data);
+  try (split; [ solve [ encode ] | ]).
+
+Ltac pure_call_VClo :=
+  apply pure_enter_call_VClo; simpl; apply pure_EvalRetThrow.
+
+(* [pure_simp] expects a goal of the form [pure m φ]. It simplifies
+   [m] into [m'], if possible, and leaves the goal [pure m' φ]. *)
+
+Ltac pure_simp :=
+  eapply pure_simp; [ simp_really |].
+
+(* -------------------------------------------------------------------------- *)
+
+(* pure0 leaves zero subgoal. *)
+(* pure1 leaves one subgoal, which may have an arbitrary shape. *)
+
+Ltac pure0 :=
+  try pure_simp;
+  first [
+
+    pure_ret; [
+      (* goal: [φ x] *)
+      pure_close
+    ]
+
+  | simple eapply pure_call; [
+      (* goal: [v = #x] *)
+      solve [encode]
+    | (* goal: [pure (call #x) φ] *)
+      pure_close
+    ]
+
+  | simple eapply pure_call_consequence; [
+      (* goal: [v = #x] *)
+      solve [encode]
+      (* goal: [pure (call #x) φ] *)
+    | solve [eauto with pure_specs]
+      (* goal: [∀ x, φ x → φ' x] *)
+    | pure_close
+    ]
+
+  | simple eapply pure_bind_as_bool; [ pure0 | beta; intros; pure0 ]
+  | simple eapply pure_bind_as_int ; [ pure0 | beta; intros; pure0 ]
+  | simple eapply pure_bind        ; [ pure0 | beta; intros; pure0 ]
+  | simple eapply pure_try         ; [ pure0 | beta; intros; pure0 ]
+
+  | pure_close
+
+  ]
+
+with pure1 :=
+  try pure_simp;
+  first [
+
+    pure_ret (* residual goal: [φ x] *)
+
+  | simple eapply pure_call_consequence; [
+      (* goal: [v = #x] *)
+      solve [encode]
+      (* goal: [pure (call #x) φ] *)
+    | solve [eauto with pure_specs]
+      (* residual goal: [∀ x, φ x → φ' x] *)
+    | beta
+    ]
+
+  | simple eapply pure_call; [
+      (* goal: [v = #x] *)
+      solve [encode]
+    | (* residual goal: [pure (call #x) φ] *)
+      idtac
+    ]
+
+  | simple eapply pure_bind_as_bool; [ pure0 | (* residual goal *) beta ]
+  | simple eapply pure_bind_as_int ; [ pure0 | (* residual goal *) beta ]
+  | simple eapply pure_bind        ; [ pure0 | (* residual goal *) beta ]
+  | simple eapply pure_try         ; [ pure0 | (* residual goal *) beta ]
+
+  | idtac (* residual goal *)
+
+  ]
+
+with pure_close :=
+  solve [ eauto with pure_specs representable ].
+
+Ltac pure1_call_step :=
+  first [
+    eapply pure_enter_call_VClo
+  | eapply pure_enter_call_VCloRec
+  ].
+
+Ltac pure_enter :=
+  pure1_call_step;
+  pure1.
+
+Ltac pure_specify x φ :=
+  lazymatch goal with
+  | |- pure (bind (ret (?δ ++ _, ?δ ++ _)) _) _ =>
+      let o := eval cbn in (lookup_name δ x) in
+      lazymatch o with ret ?v =>
+        let h := fresh in
+        assert (φ v) as h; [| revert h; generalize v ]
+      end
+  end.
+
+(* It is debatable in which order the two premises of the lemma [pure_call]
+   should be attacked. The premise [v'2 = #x] may seem easy to solve (this
+   is the job of the tactic [encode]) so one may wish to solve it first.
+   This offers the advantage of instantiating [x] immediately, so [x] is
+   known when we try to prove that the call is permitted -- which may
+   involve proving that a precondition holds.
+
+   However, solving [v'2 = #x] can involve guessing some types (e.g., the
+   type of an empty list), and we have used [Hint Mode] in encode.v to
+   forbid this. So, it can also be preferable to first solve the premise
+   [pure (call v1 #x) φ]. Doing so can allow us to instantiate these types
+   in a correct way.
+
+   One might wish to try both approaches in sequence, but waiting until
+   [encode] fails is very slow (several seconds).
+
+   One might also wish to do a bit of both: that is, first apply some lemma
+   [L] to the subgoal [pure (call v1 #x) φ], then solve [v'2 = #x], then
+   attack the proof obligations created by applying the lemma [L]. *)
+
+Create HintDb pure_specs.
+
+(* TODO may be unused *)
+Ltac pure_call :=
+  first [
+    simple eapply pure_call; [ solve [encode] | solve [eauto with pure_specs] ]
+  | simple eapply pure_consequence; [
+      simple eapply pure_call; [ solve [encode] | eauto with pure_specs ]
+    | cbn ]
+  ].
+
+Ltac pure_enter_and_abstract :=
+  lazymatch goal with |- pure (call ?v _) _ =>
+    (* First, expand [call] away. *)
+    pure1_call_step;
+    normalize;
+    (* Second, abstract away the closure (of which there are typically
+       several occurrences in the hypotheses and goal), replacing it
+       with an abstract value. This ensures that we cannot step into
+       recursive calls. *)
+    generalize dependent v
+  end.
+
+(* -------------------------------------------------------------------------- *)
+
+(* Evaluate an [eval] by repeatedly changing [eval] into [eval'] *)
+Ltac simp_evaluate :=
+  simpl; repeat (rewrite eval_eval'; simpl).
+
+(* TODO the following tactics seem redundant with the symbolic execution
+        tactics, [simp] and friends. Avoid duplication. *)
+
+(* On a goal of the form [pure (Stop CEval x k ko) φ], evaluate the call by:
+   stepping through the [Stop] with the appropriate advance_SimpEval lemma,
+   using [simp_evaluate] under the resulting pure *)
+Ltac pure_evaluate :=
+  (lazymatch goal with
+   | |- pure (Stop CEval _ _ _) _ =>
+       eapply pure_simp; [
+         first [
+           apply advance_SimpEvalRetThrow
+         | apply advance_SimpEvalThrow
+         | apply advance_SimpEval
+         ]
+       | apply SimpReflexive
+       ]
+   | _ => idtac
+   end);
+  eapply pure_simp; [simp_evaluate; apply SimpReflexive|].
+
+Ltac SimpParRet :=
+  first [
+    apply SimpParRetRet
+  | apply SimpParRetLeftThrow
+  | apply SimpParRetRightThrow
+  | apply SimpParRetLeft
+  | apply SimpParRetRight
+  ].
+
+Ltac pureParRet :=
+  eapply pure_simp; first SimpParRet; simpl.
+
+(* -------------------------------------------------------------------------- *)
+
+(* Dummy proposition with one constructor *)
+Inductive BLOCK := block.
+
+(* Tranform a goal of the form [H1 -> H2 -> ... -> BLOCK -> G] into
+   [H1 /\ H2 /\ ... -> G] *)
+Ltac conj_until_BLOCK b :=
+  lazymatch goal with
+  | |- BLOCK -> _ =>
+      intros _; let H := fresh in
+               pose proof (H := I); revert H
+  | |- _ -> BLOCK -> _ =>
+      let H1 := fresh in
+      intros H1 _; revert H1
+  | |- ?A -> ?B -> _ =>
+      let H1 := fresh in
+      let H2 := fresh in
+      let H3 := fresh in
+      intros H1 H2; pose proof (H3 := conj H2 H1);
+      revert H3;
+      match b with
+      | true => clear H1; conj_until_BLOCK true
+      | false => conj_until_BLOCK true
+      end
+  end.
+
+(* Given a tuple (or single term), move all hypotheses depending on elements
+   of the tuple (or single term) into the goal *)
+Ltac generalize_tuple t :=
+  match t with
+  | pair ?x ?y =>
+      generalize dependent y; intro;
+      generalize_tuple x
+  | _ => generalize dependent t; intro
+  end.
+
+(* Given a term (or tuple of terms), move all hypotheses depending on this term
+   (or tuple of terms) into the goal as a single conjunction *)
+Ltac capture_hypotheses_aux arg :=
+  generalize (block);
+  generalize_tuple arg;
+  conj_until_BLOCK false.
+
+Tactic Notation "capture_hypotheses" constr(arg1) :=
+  capture_hypotheses_aux arg1.
+
+Tactic Notation "capture_hypotheses" constr(arg1) "as" simple_intropattern(x) :=
+  capture_hypotheses_aux arg1; intros x.
+
+Tactic Notation "capture_hypotheses" constr(arg1) constr(arg2) :=
+  capture_hypotheses_aux (arg1, arg2).
+
+Tactic Notation "capture_hypotheses" constr(arg1) constr(arg2) "as" simple_intropattern(x) :=
+  capture_hypotheses_aux (arg1, arg2); intros x.
+
+(* Automatically apply [pure_rec_call] on a goal of the form [pure m φ] *)
+Ltac pure_rec_tac arg pre Hwf :=
+  (* Eta-expand the postcondition *)
+  match goal with
+  | |- pure _ ?H =>
+      let post := fresh in
+      set (post := H); pattern arg in post; cbv delta [post]; clear post
+  end;
+  (* Apply [pure_rec_call], possibly with an explicit precondition *)
+  match pre with
+  | None =>
+      eapply pure_rec_call with (v:=arg)
+  | Some ?pre =>
+      eapply pure_rec_call with (v:=arg) (P:=pre)
+  end;
+  (* Try and solve subgoals generated by [pure_rec_call] *)
+  [ apply Hwf
+  | lazymatch pre with
+    | None =>
+        capture_hypotheses arg;
+        let HPre := fresh in intros HPre;
+        pattern arg in HPre;
+        exact HPre
+    | Some _ =>
+        subst; auto; fail
+    end
+  | ];
+  clear dependent arg; (* [pure_rec_call] deprecates the original argument *)
+  let HP := fresh "HP" in
+  let IH := fresh "IH" in
+  simpl; intros vf arg HP IH.
+
+Tactic Notation "pure_rec" constr(arg) constr(Hwf) :=
+  pure_rec_tac arg constr:(@None False) Hwf.
+
+Tactic Notation "pure_rec" constr(arg) constr(pre) constr(Hwf) :=
+  pure_rec_tac arg constr:(Some pre) Hwf.
+
+(* Automatically apply [pure_nested_call] on a goal of the form [pure m φ] *)
+Ltac pure_nested_tac arg1 arg2 pre Hwf :=
+  match goal with
+  | |- pure _ (fun c => pure _ ?H) =>
+      let post := fresh in
+      set (post := H); pattern arg1, arg2 in post; cbv delta [post]; clear post;
+      lazymatch pre with
+      | None =>
+          eapply pure_nested_call with (v1:=arg1) (v2:=arg2)
+      | Some ?pre =>
+          eapply pure_nested_call with (v1:=arg1) (v2:=arg2) (P:=pre)
+      end;
+      [ reflexivity
+      | simpl; rewrite eval_eval'; reflexivity
+      | apply Hwf
+      | lazymatch pre with
+          None =>
+            capture_hypotheses arg1 arg2;
+            let HPre := fresh in intros HPre;
+                                 pattern arg1, arg2 in HPre;
+                                 exact HPre
+        | Some _ =>
+            auto
+        end
+      | ];
+      let HP := fresh "HP" in
+      let IH := fresh "IH" in
+      clear dependent arg1 arg2;
+      simpl; intros vf arg1 arg2 HP IH
+  end.
+
+Tactic Notation "pure_nested" constr(arg1) constr(arg2) constr(Hwf) :=
+  pure_nested_tac arg1 arg2 constr:(@None False) Hwf.
+
+Tactic Notation "pure_nested" constr(arg1) constr(arg2)
+  constr(pre) constr(Hwf) :=
+  pure_nested_tac arg1 arg2 constr:(Some pre) Hwf.
+
+(* -------------------------------------------------------------------------- *)
+
+Module Tac.
+  Import Ltac2.
+
+  Ltac2 eta_post' (arg : constr list) :=
+    lazy_match! goal with
+    | [ |- pure _ ?φ ] =>
+        let post := Fresh.in_goal @post in
+        set ($post := $φ);
+        Std.pattern (List.map (fun x => (x, Std.AllOccurrences)) arg)
+          { Std.on_hyps := Some [(post, Std.AllOccurrences, Std.InHyp)];
+                           Std.on_concl := Std.NoOccurrences };
+        cbv delta [&post];
+        clear $post
+    end.
+
+  Import Constr.Unsafe.
+
+  Ltac2 eta_post'' (arg : Ltac1.t) :=
+    let arg := Option.get (Ltac1.to_list arg) in
+    let arg := List.map (fun x => Option.get (Ltac1.to_constr x)) arg in
+    eta_post' arg.
+
+  Ltac eta_post arg :=
+    let f := ltac2:(arg |- eta_post'' arg) in
+    f arg.
+
+  Tactic Notation "eta_post" constr_list(arg) :=
+    let f := ltac2:(arg |- eta_post'' arg) in
+    f arg.
+
+  Ltac2 eta_tuple_aux t :=
+    let rec aux t :=
+      lazy_match! t with
+      | pair ?x ?y =>
+          let l := aux x in
+          List.append l [y]
+      | ?single => [single]
+      end
+    in
+    let arg_list := aux t in
+    eta_post' arg_list.
+
+  Ltac2 eta_tuple_aux_interface (arg : Ltac1.t) :=
+    let arg := Option.get (Ltac1.to_constr arg) in
+    eta_tuple_aux arg.
+
+  Tactic Notation "eta_tuple" constr(arg) :=
+    let f := ltac2:(arg |- eta_tuple_aux_interface arg) in
+    f arg.
+
+End Tac.
