coq-osiris/theories/proofmode/simp_tactics.v
@@ -1,274 +1,923 @@
 From osiris Require Import base.
 From osiris.lang Require Import lang.
 From osiris.semantics Require Import semantics.
-From osiris.proofmode Require Import simp pure_hoare simp_eval.
-From Ltac2 Require Ltac2.
+From osiris.proofmode Require Import equality.
+From osiris.proofmode Require Import specifications.
 
-(* This file contains tactics intended for use during hoare-style proofs of pure
-   programs. These range from symbolic execution to tactics designed to aid
-   the application of single lemmas.
+(* A pure computation is terminating, deterministic, and does not use
+   mutable state. *)
 
-   Very Work-In-Progress and subject to change (10/12/2023) *)
+(* This file offers lemmas and tactics that help simplify computations,
+   that is, solve goals of the form [simp m1 ?m2]. *)
+
+(* -------------------------------------------------------------------------- *)
+
+(* We do not want to unfold [val_as_bool] into a case analysis; that would be
+   counter-productive, and could cause the tactics below to diverge.
+
+   Note that [val_as_bool] is more problematic than [val_as_int] because
+   integer values have their own tag [VInt], whereas Boolean values do not.
+   [VBool] is just sugar, not a genuine tag. *)
+
+Global Opaque val_as_bool.
+
+(* -------------------------------------------------------------------------- *)
+
+(* Opacity control. *)
+
+(* [force_unfold_at_1 x] unfolds the first occurrence of [x]
+   and works even if [x] is opaque. *)
+
+Ltac force_unfold_at_1 x :=
+  with_strategy transparent [x] unfold x at 1.
+
+(* [force_unfold x] unfolds all occurrences of [x]
+   and works even if [x] is opaque. *)
+
+Ltac force_unfold x :=
+  with_strategy transparent [x] unfold x.
+
+(* -------------------------------------------------------------------------- *)
+
+(* The following lemmas are reasoning rules for goals of the form [simp _ _]. *)
+
+(* They are used by the tactics that follow. *)
+
+(* [prove_simp_ret] reduces the goal to an equality between values [a1 = a2]. *)
+
+Lemma prove_simp_ret {A E} (a1 a2 : A) :
+  a1 = a2 →
+  simp (ret a1 : micro A E) (ret a2).
+Proof.
+  intros. subst. eauto with simp.
+Qed.
+
+(* These lemmas are trivial. They could be replaced by nested applications of
+   constructors, possibly complemented with [rewrite] steps. Using lemmas is
+   somewhat more robust and should give rise to smaller proof terms. *)
+
+Lemma simp_reflexive {A E} (m1 m2 : micro A E) :
+  m1 = m2 →
+  simp m1 m2.
+Proof.
+  intros. subst. eauto with simp.
+Qed.
+
+Lemma simp_reflexive_ret {A E} (m1 : micro A E) a2 :
+  m1 = ret a2 →
+  simp m1 (ret a2).
+Proof.
+  intros. subst. eauto with simp.
+Qed.
+
+Lemma advance_simp_let η δ bs e m2 :
+  simp (eval_bindings η bs) (ret δ) ->
+  simp (eval (δ ++ η) e) m2 ->
+  simp (eval η (ELet bs e)) m2.
+Proof.
+  intros. rewrite eval_eval'; simpl.
+  eapply prove_simp_bind; eauto.
+Qed.
+
+Lemma advance_simp_letrec η δ rbs e m2 :
+  eval_rec_bindings η rbs = δ ->
+  simp (eval (δ ++ η) e) m2 ->
+  simp (eval η (ELetRec rbs e)) m2.
+Proof.
+  intros Hevalrb ?.
+  rewrite eval_eval'; simpl.
+  by rewrite Hevalrb.
+Qed.
+
+Lemma advance_simp_ilet η1 η2 δ bs sitems m2 :
+  simp (eval_bindings η1 bs) (ret δ) ->
+  simp (eval_sitems (δ ++ η1, δ ++ η2) sitems) m2 ->
+  simp (eval_sitems (η1, η2) ((ILet bs) :: sitems)) m2.
+Proof.
+  intros.
+  eapply prove_simp_bind; last eassumption.
+  eapply prove_simp_bind; [ eassumption | apply SimpReflexive ].
+Qed.
+
+Lemma advance_simp_iletrec η1 η2 δ rbs sitems m2 :
+  eval_rec_bindings η1 rbs = δ ->
+  simp (eval_sitems (δ ++ η1, δ ++ η2) sitems) m2 ->
+  simp (eval_sitems (η1, η2) ((ILetRec rbs) :: sitems)) m2.
+Proof.
+  intros Heq ?.
+  eapply prove_simp_bind; last eassumption.
+  simpl; rewrite Heq; apply SimpReflexive.
+Qed.
+
+Lemma advance_simp_imodule η1 η2 m v me sitems m2 :
+  simp (eval_mexpr η1 me) (ret v) ->
+  simp (eval_sitems ([(m, v)] ++ η1, [(m, v)] ++ η2) sitems) m2 ->
+  simp (eval_sitems (η1, η2) ((IModule m me) :: sitems)) m2.
+Proof.
+  intros.
+  eapply prove_simp_bind; last eassumption.
+  { eapply prove_simp_bind; first eassumption.
+    apply SimpReflexive. }
+Qed.
+
+Lemma advance_simp_mexpr η δ δ' sitems :
+  simp (eval_sitems (η, []) sitems) (Ret (δ', δ)) ->
+  simp (eval_mexpr η (MStruct sitems)) (Ret (VStruct δ)).
+Proof.
+  intros Hsimp.
+  eapply prove_simp_bind. { apply Hsimp. }
+  apply SimpReflexive.
+Qed.
+
+Lemma advance_SimpEval {A E} η e (k : val → micro A E) z m' :
+  simp (try (eval η e) k z) m' →
+  simp (Stop CEval (η, e) k z) m'.
+Proof.
+  eauto with simp.
+Qed.
+
+Lemma advance_SimpEvalThrow {A} η e (k : val → micro A void) m' :
+  simp (bind (eval η e) k) m' →
+  simp (Stop CEval (η, e) k throw) m'.
+Proof.
+  rewrite bind_as_try. eauto with simp.
+Qed.
+
+Lemma advance_SimpEvalRetThrow η e m' :
+  simp (eval η e) m' ->
+  simp (Stop CEval (η, e) ret throw) m'.
+Proof.
+  intros.
+  by apply advance_SimpEvalThrow; rewrite bind_ret_right.
+Qed.
+
+Lemma advance_SimpEvalRetThrow' η e m' :
+  simp (eval η e) m' →
+  simp (stop CEval (η, e)) m'.
+Proof.
+  unfold stop. eauto using advance_SimpEvalRetThrow.
+Qed.
+
+Lemma advance_SimpLoop {A E} η x i1 i2 e (k : val → micro A E) z m' :
+  simp (try (loop η x i1 i2 e) k z) m' →
+  simp (Stop CLoop (η, x, i1, i2, e) k z) m'.
+Proof.
+  eauto with simp.
+Qed.
+
+Lemma advance_SimpLoopThrow {A} η x i1 i2 e (k : val → micro A void) m' :
+  simp (bind (loop η x i1 i2 e) k) m' →
+  simp (Stop CLoop (η, x, i1, i2, e) k throw) m'.
+Proof.
+  rewrite bind_as_try. eauto with simp.
+Qed.
+
+Lemma advance_SimpChooseAgree {A B E' E} m1 m2 m (k : A → micro B E) (z : E' → _) m' :
+  simp m1 m →
+  simp m2 m →
+  simp (try m k z) m' →
+  simp (Choose m1 m2 k z) m'.
+Proof.
+  eauto with simp.
+Qed.
+
+Lemma advance_simp_choose {A E} (m1 m2 : micro A E) m' :
+  simp m1 m' →
+  simp m2 m' →
+  simp (choose m1 m2) m'.
+Proof.
+  intros. eapply advance_SimpChooseAgree; eauto.
+  rewrite try_ret_right. eauto with simp.
+Qed.
+
+Lemma advance_SimpBind {A B E} m1 m2 (f : A → micro B E) m' :
+  simp m1 m2 →
+  simp (bind m2 f) m' →
+  simp (bind m1 f) m'.
+Proof.
+  eauto using simp_bind with simp.
+Qed.
+
+Lemma advance_SimpTry {A B E' E} m1 m2 (f : A → micro B E) (h : E' → _) m' :
+  simp m1 m2 →
+  simp (try m2 f h) m' →
+  simp (try m1 f h) m'.
+Proof.
+  eauto using simp_try with simp.
+Qed.
+
+Lemma advance_SimpParRetRet {A1 A2 A E' E}
+  a1 a2 (k : A1 * A2 → micro A E) (z : E' → _) m'
+:
+  simp (k (a1, a2)) m' →
+  simp (Par (Ret a1) (Ret a2) k z) m'.
+Proof.
+  eauto using SimpParRetRet with simp.
+Qed.
+
+Lemma advance_SimpParRetLeft {A1 A2 A E' E}
+  a1 m2 (k : A1 * A2 → micro A E) (h : E' → _) m'
+:
+  simp (try m2 (λ v2, k (a1, v2)) h) m' →
+  simp (Par (Ret a1) m2 k h) m'.
+Proof.
+  eauto with simp.
+Qed.
+
+Lemma advance_SimpParRetRight {A1 A2 A E' E}
+  m1 a2 (k : A1 * A2 → micro A E) (h : E' → _) m'
+:
+  simp (try m1 (λ v1, k (v1, a2)) h) m' →
+  simp (Par m1 (Ret a2) k h) m'.
+Proof.
+  eauto with simp.
+Qed.
+
+Lemma advance_SimpParRetLeftThrow {A1 A2 A E}
+  a1 m2 (k : A1 * A2 → micro A E) m'
+:
+  simp (v2 ← m2 ; k (a1, v2)) m' →
+  simp (Par (Ret a1) m2 k throw) m'.
+Proof.
+  rewrite bind_as_try. eauto using advance_SimpParRetLeft.
+Qed.
+
+Lemma advance_SimpParRetRightThrow {A1 A2 A E}
+  m1 a2 (k : A1 * A2 → micro A E) m'
+:
+  simp (v1 ← m1 ; k (v1, a2)) m' →
+  simp (Par m1 (Ret a2) k throw) m'.
+Proof.
+  rewrite bind_as_try. eauto using advance_SimpParRetRight.
+Qed.
+
+Lemma advance_SimpPar {A1 A2 A E' E}
+  m1 m'1 m2 m'2 (k : A1 * A2 → micro A E) (z : E' → _) m'
+:
+  simp m1 m'1 →
+  simp m2 m'2 →
+  simp (Par m'1 m'2 k z) m' →
+  simp (Par m1 m2 k z) m'.
+Proof.
+  eauto with simp.
+Qed.
+
+(* -------------------------------------------------------------------------- *)
+
+(* More lemmas for use by the tactics that follow. *)
+
+(* [val_as_bool] is opaque. to deal with it, we use the following lemmas. *)
+
+Lemma val_as_bool_VTrue :
+  val_as_bool VTrue = ret true.
+Proof.
+  reflexivity.
+Qed.
+
+Lemma val_as_bool_VFalse :
+  val_as_bool VFalse = ret false.
+Proof.
+  reflexivity.
+Qed.
+
+Lemma val_as_bool_VBool b :
+  val_as_bool (VBool b) = ret b.
+Proof.
+  destruct b; reflexivity.
+Qed.
+
+Lemma advance_simp_val_as_bool_VTrue m' :
+  simp (ret true) m' →
+  simp (val_as_bool VTrue) m'.
+Proof.
+  rewrite val_as_bool_VTrue. tauto.
+Qed.
+
+Lemma advance_simp_val_as_bool_VFalse m' :
+  simp (ret false) m' →
+  simp (val_as_bool VFalse) m'.
+Proof.
+  rewrite val_as_bool_VFalse. tauto.
+Qed.
+
+Lemma advance_simp_val_as_bool_VBool b m' :
+  simp (ret b) m' →
+  simp (val_as_bool (VBool b)) m'.
+Proof.
+  rewrite val_as_bool_VBool. tauto.
+Qed.
+
+Lemma advance_simp_pure_spec_val_as_struct `{Σ: iprop.gFunctors} v a l P :
+  @pure_spec Σ val (SpecModule a l P) v →
+  simp (val_as_struct v) (Ret (val_as_struct_total v)).
+Proof.
+  intros H. pose proof H as (?&->&_).
+  by erewrite pure_spec_val_as_struct.
+Qed.
+
+Lemma advance_simp_is_module_val_as_struct v Λ :
+  is_module Λ v →
+  simp (val_as_struct v) (Ret (val_as_struct_total v)).
+Proof. intros?. by erewrite is_module_val_of_struct. Qed.
+
+
+Lemma advance_simp_is_module_lookup_name v Λ n :
+  is_module Λ v →
+  In n Λ →
+  simp (lookup_name (val_as_struct_total v) n)
+       (Ret (lookup_name_total (val_as_struct_total v) n)).
+Proof.
+  intros??.
+  by erewrite is_module_lookup_name_total.
+Qed.
+
+Lemma advance_simp_pure_spec_lookup_name `{Σ : iprop.gFunctors} v a l P n :
+  @pure_spec Σ val (SpecModule a l P) v →
+  In n (List.map fst l) →
+  simp (lookup_name (val_as_struct_total v) n)
+       (Ret (lookup_name_total (val_as_struct_total v) n)).
+Proof.
+  intros H?. pose proof H as (?&->&_).
+  by erewrite pure_spec_lookup_total.
+Qed.
+
+(* -------------------------------------------------------------------------- *)
+
+(* More lemmas for use by the tactics that follow. *)
+
+(* This lemma gives the user a chance to prove that the actual argument
+   [v'2] is in fact the encoding of some value [x]. The subgoal [v'2 = #x]
+   is typically solved by the tactic [encode]. Solving this subgoal
+   instantiates both the metavariable [x] and the metavariable [X], which is
+   the type of [x]. *)
+
+Lemma simp_call `{Encode X} v1 v'2 (x : X) m' :
+  v'2 = #x →
+  simp (call v1 #x) m' →
+  simp (call v1 v'2) m'.
+Proof.
+  intros. subst. eauto.
+Qed.
+
+(* The following two lemmas paraphrase the definition of [call] in eval.v.
+   When applied to a goal of the form [simp (call v1 v2) _] where [v1] is a
+   concrete closure (as opposed to a rigid metavariable), they step into the
+   call.
+
+   If [eapply] is used, as opposed to [simple eapply], then a definition can
+   be unfolded on the fly: that is, the lemma can be applied to a goal of
+   the form [simp (call c v2) m] where [c] is the name of a Coq toplevel
+   definition.
+
+   The trouble with [eapply], though, is that it does not respect opacity
+   (i.e., it can unfold both transparent and opaque definitions).
+   Furthermore, somewhat surprisingly, it can unfold and simplify further
+   than is strictly necessary for the lemma to be applicable. *)
+
+Lemma simp_enter_call_VClo η a v2 m :
+  simp (acall η a v2) m →
+  simp (call (VClo η a) v2) m.
+Proof.
+  tauto.
+Qed.
+
+Lemma simp_enter_call_VCloRec η rbs g v2 m :
+  simp (
+    let δ := eval_rec_bindings η rbs in
+    let η := δ ++ η in
+    a ← lookup_rec_bindings rbs g ;
+    acall η a v2
+  ) m →
+  simp (call (VCloRec η rbs g) v2) m.
+Proof.
+  tauto.
+Qed.
+
+(* This lemma replaces [eval] with [eval'] at the root of the goal. *)
+
+Lemma advance_simp_eval η e m' :
+  simp (eval' η e) m' →
+  simp (eval  η e) m'.
+Proof.
+  rewrite eval_eval'. tauto.
+Qed.
+
+Lemma advance_SimpEvalEAssert η e :
+  simp (eval η e) (ret #true) →
+  simp (eval η (EAssert e)) ok.
+Proof.
+  intros.
+  eapply advance_simp_eval. simpl eval'.
+  (* Because of [choose], the runtime test may be skipped or executed.
+     If it is skipped, then the result is immediate. If it is executed,
+     then the assumption that [e] evaluates to [true] is exploited. *)
+  eapply advance_simp_choose.
+  { apply SimpReflexive. }
+  unfold as_bool.
+  rewrite bind_bind.
+  eapply prove_simp_bind.
+  { eauto. }
+  eapply SimpReflexive.
+Qed.
+
+(* -------------------------------------------------------------------------- *)
+
+(* More lemmas for use by the tactics that follow. *)
+
+(* The following lemmas paraphrase the rewrite rules [ret_bind], [bind_ret],
+   etc., and force the rule to be applied at the root of the goal. This is
+   both safe and efficient (there is no need to scan the whole term). *)
+
+Lemma advance_simp_bind_ret {A B E} (a : A) (f : A → micro B E) m' :
+  simp (f a) m' →
+  simp (bind (ret a) f) m'.
+Proof.
+  simpl bind. tauto.
+Qed.
+
+Lemma advance_simp_bind_ret_right {A E} (m : micro A E) m' :
+  simp m m' →
+  simp (bind m ret) m'.
+Proof.
+  rewrite bind_ret_right. eauto.
+Qed.
+
+Lemma advance_simp_try_ret {A B E' E} (a : A) (f : A → micro B E) (h : E' → _) m' :
+  simp (f a) m' →
+  simp (try (ret a) f h) m'.
+Proof.
+  rewrite try_ret. tauto.
+Qed.
+
+Lemma advance_simp_try_throw {A B E' E} x' (f : A → micro B E) (h : E' → _) m' :
+  simp (h x') m' →
+  simp (try (throw x') f h) m'.
+Proof.
+  simpl try. tauto.
+Qed.
+
+Lemma advance_simp_bind_as_try {A B E} m (f : A → micro B E) m' :
+  simp (bind m f) m' →
+  simp (try m f throw) m'.
+Proof.
+  rewrite bind_as_try. tauto.
+Qed.
+
+Lemma advance_simp_bind_bind
+  {A B C E} (m : micro A E) (f : A → micro B E) (g : B → micro C E) m' :
+  simp (bind m (λ a, bind (f a) g)) m' →
+  simp (bind (bind m f) g) m'.
+Proof.
+  rewrite bind_bind. tauto.
+Qed.
+
+Lemma advance_simp_bind_try {A B C E' E}
+  (m : micro A E') (f : A → micro B E) (g : B → micro C E) (h : E' → _) m' :
+  simp (try m (λ a, bind (f a) g) (λ y, bind (h y) g)) m' →
+  simp (bind (try m f h) g) m'.
+Proof.
+  rewrite bind_try. tauto.
+Qed.
+
+Lemma advance_simp_try_bind {A B C E}
+  m (f : A → micro B E) (g : B → micro C E) h m'
+:
+  simp (try m (λ y, try (f y) g h) h) m' →
+  simp (try (bind m f) g h) m'.
+Proof.
+  rewrite try_bind. tauto.
+Qed.
+
+Lemma advance_simp_try_try {A B C E'' E' E}
+  (m : micro A E'') (f : A → micro B E') (g : B → micro C E) h h' m' :
+  simp (try m (λ y, try (f y) g h') (λ y, try (h y) g h')) m' →
+  simp (try (try m f h) g h') m'.
+Proof.
+  rewrite try_try. tauto.
+Qed.
+
+(* -------------------------------------------------------------------------- *)
+
+(* Some properties of integer arithmetic. *)
+
+(* [Is_true] is implicit in these statements. Its type is [bool → Prop]. *)
+
+Lemma Zeq_spec (x y : Z) :
+  (x =? y) ↔ (x = y).
+Proof.
+  rewrite Is_true_true, Z.eqb_eq. tauto.
+Qed.
+
+Lemma Zne_spec (x y : Z) :
+  negb (x =? y) ↔ x ≠ y.
+Proof.
+  rewrite negb_True, Zeq_spec. tauto.
+Qed.
+
+Lemma Zlt_spec (x y : Z) :
+  (x <? y) ↔ (x < y).
+Proof.
+  rewrite Is_true_true, Zlt_is_lt_bool. tauto.
+Qed.
+
+Lemma Zle_spec (x y : Z) :
+  negb (y <? x) ↔ x ≤ y.
+Proof.
+  rewrite negb_True, Zlt_spec. lia.
+Qed.
 
 (* -------------------------------------------------------------------------- *)
 
 (* Tactics. *)
 
-(* TODO reduce just beta-redexes in the goal (possibly under ∀ and →) *)
+(* We systematically use [simply eapply] as opposed to [eapply], because
+   the latter does not respect opacity. (It is stronger than we wish.) *)
 
-Ltac beta :=
-  cbn beta.
+Create HintDb simp_specs.
 
-Goal (forall l : list nat,
-         l = [] ->
-         (λ (x : bool), negb x = ((λ (x : bool), x) false)) true).
-Proof.
-  beta. reflexivity.
-Qed.
+(* [simp_ret] expects of the goal of the form [simp (ret ?a1) (ret ?a2)].
+   It reduces this goal to the equality [a1 = a2], and attempts to prove
+   this equality. It leaves zero or one subgoal. *)
 
-(* [remove_deco] is used by subsequent tactics when we want to match on an
-   expression under a decoration in a goal. *)
+Ltac simp_ret :=
+  simple eapply prove_simp_ret; [ eauto with encode equality ].
+(* TODO limit search depth? *)
 
-Ltac remove_deco :=
-  lazymatch goal with
-  | |- pure (eval _ (deco _ _)) _ => unfold deco at 1; simpl
-  | _ => idtac
-  end.
+(* The tactic [normalize] attempts to reduce and normalize the goal.
+   It is used (as sparingly as possible) by the tactics that follow. *)
 
-(* Remove any local environment definitions. *)
+Ltac normalize :=
+  cbn.
 
-Ltac clear_abstracted_env :=
-  repeat (match goal with
-          | η := _ : list (var * val) |- _ => subst η
-          end).
+(* [simp_close] solves a goal of the form [simp m1 m2] using reflexivity.
 
-(* [abstract_env] expects a goal of the form [pure (eval η e) φ]. It creates a
-   local definition for the environment [η]. *)
+   If reflexivity cannot solve the goal, then [simp_close] fails. *)
 
-Ltac abstract_env :=
-  lazymatch goal with
-  | |- pure (eval ?η _) _ =>
-      clear_abstracted_env;
-      match goal with
-      | |- pure (eval ?η _) _ =>
-          let η0 := fresh "η" in
-          set η as η0
-      end
-  | _ => idtac
-  end.
-
-Ltac extend_env :=
-  match goal with
-  | |- forall (η : env), η = _ -> _ =>
-      intros ? ->
-  | _ => idtac
-  end.
-
-(* -------------------------------------------------------------------------- *)
-
-(* [pure_ret] expects a goal of the form [pure (ret v) φ]. It applies
-   the lemma [pure_ret], solves the subgoal [v = #x], and leaves just
-   the subgoal [φ x], which it simplifies. *)
-
-Ltac pure_ret :=
-  remove_deco;
-  match goal with
-  | |- pure (ret ?v) ?φ =>
-      match type of φ with
-      | val -> Prop =>
-          simple eapply pure_ret; [ rewrite <- solve_encode_val; reflexivity | beta]
-      | _ =>
-          simple eapply pure_ret; [ solve [ encode ] | beta ]
-      end
-  end.
-
-(* [pure_path] expects a goal of the form [pure (eval η (EPath x)) φ]. It applies
-   the lemma [pure_eval_path], asks Coq to compute the lookup in the environment,
-   and, assuming that the lookup succeeds, calls pure_ret on the result. *)
-
-Ltac pure_path :=
-  remove_deco;
-  eapply pure_eval_path; simpl lookup_path;
-  match goal with
-  | H : lookup_name ?η ?path = ret ?res |- pure (lookup_name ?η ?path) _ =>
-      rewrite H
-  | _ => idtac
-  end;
-  pure_ret.
-
-(* [pure_const] expects a goal of the form [pure (eval η (EConstant x)) φ].
-   It applies the lemma [pure_eval_const], solves the subgoal [VConstant c = #x],
-   and leaves the subgoal [φ x]. *)
-
-Ltac pure_const :=
-  remove_deco;
-  match goal with
-  | |- pure (eval ?η (EConstant ?c)) ?ψ =>
-      match type of ψ with
-      | val -> Prop =>
-          simple eapply pure_eval_const; [ rewrite <- solve_encode_val; reflexivity | ]
-      | _ =>
-          simple eapply pure_eval_const; [ solve [ encode ] | ]
-      end
-  end.
-
-Local Open Scope nat.
-
-Ltac pure_data :=
-  remove_deco;
-  simpl;
-  match goal with
-  | |- pure (eval _ (EData ?c (ETuple ?args))) _ =>
-      match eval cbn in (length args) with
-      | 0 => pure_const
-      | 1 => eapply pure_eval_data1
-      | 2 => eapply pure_eval_data2; eapply pure_eval_pair
-      | 3 => eapply pure_eval_data3; eapply pure_eval_triple
-      | 4 => eapply pure_eval_data4
-      (* TODO: make a higher-order version of pure_eval_pair *)
-      | _ => fail "Not implemented for this arity"
-      end
-  end;
-  repeat (pure_path || pure_const || pure_data);
-  try (split; [ solve [ encode ] | ]).
-
-Ltac pure_call_VClo :=
-  apply pure_enter_call_VClo; simpl; apply pure_EvalRetThrow.
-
-(* [pure_simp] expects a goal of the form [pure m φ]. It simplifies
-   [m] into [m'], if possible, and leaves the goal [pure m' φ]. *)
-
-Ltac pure_simp :=
-  eapply pure_simp; [ simp_really |].
-
-(* -------------------------------------------------------------------------- *)
-
-(* pure0 leaves zero subgoal. *)
-(* pure1 leaves one subgoal, which may have an arbitrary shape. *)
-
-Ltac pure0 :=
-  try pure_simp;
-  first [
-
-    pure_ret; [
-      (* goal: [φ x] *)
-      pure_close
-    ]
-
-  | simple eapply pure_call; [
-      (* goal: [v = #x] *)
-      solve [encode]
-    | (* goal: [pure (call #x) φ] *)
-      pure_close
-    ]
-
-  | simple eapply pure_call_consequence; [
-      (* goal: [v = #x] *)
-      solve [encode]
-      (* goal: [pure (call #x) φ] *)
-    | solve [eauto with pure_specs]
-      (* goal: [∀ x, φ x → φ' x] *)
-    | pure_close
-    ]
-
-  | simple eapply pure_bind_as_bool; [ pure0 | beta; intros; pure0 ]
-  | simple eapply pure_bind_as_int ; [ pure0 | beta; intros; pure0 ]
-  | simple eapply pure_bind        ; [ pure0 | beta; intros; pure0 ]
-  | simple eapply pure_try         ; [ pure0 | beta; intros; pure0 ]
-
-  | pure_close
-
-  ]
-
-with pure1 :=
-  try pure_simp;
-  first [
-
-    pure_ret (* residual goal: [φ x] *)
-
-  | simple eapply pure_call_consequence; [
-      (* goal: [v = #x] *)
-      solve [encode]
-      (* goal: [pure (call #x) φ] *)
-    | solve [eauto with pure_specs]
-      (* residual goal: [∀ x, φ x → φ' x] *)
-    | beta
-    ]
-
-  | simple eapply pure_call; [
-      (* goal: [v = #x] *)
-      solve [encode]
-    | (* residual goal: [pure (call #x) φ] *)
-      idtac
-    ]
-
-  | simple eapply pure_bind_as_bool; [ pure0 | (* residual goal *) beta ]
-  | simple eapply pure_bind_as_int ; [ pure0 | (* residual goal *) beta ]
-  | simple eapply pure_bind        ; [ pure0 | (* residual goal *) beta ]
-  | simple eapply pure_try         ; [ pure0 | (* residual goal *) beta ]
-
-  | idtac (* residual goal *)
-
-  ]
-
-with pure_close :=
-  solve [ eauto with pure_specs representable ].
-
-Ltac pure1_call_step :=
-  first [
-    eapply pure_enter_call_VClo
-  | eapply pure_enter_call_VCloRec
+Ltac simp_close :=
+  solve [
+    simple eapply SimpReflexive
+  | simp_ret
   ].
 
-Ltac pure_enter :=
-  pure1_call_step;
-  pure1.
+(* [simp_solve_eauto] solves a goal of the form [simp m _].
 
-Ltac pure_specify x φ :=
-  lazymatch goal with
-  | |- pure (bind (ret (?δ ++ _, ?δ ++ _)) _) _ =>
-      let o := eval cbn in (lookup_name δ x) in
-      lazymatch o with ret ?v =>
-        let h := fresh in
-        assert (φ v) as h; [| revert h; generalize v ]
+   The tactic exploits whatever hypotheses are present in the context and in
+   the hint database [simp_specs]. Of course the lemma [SimpReflexive] must
+   not appear in this database; we want to make real progress.
+
+   [m] is typically of the form [call v #x] or perhaps [eval η e]. *)
+
+Ltac simp_solve_eauto :=
+  solve [ eauto with simp_specs encode typeclass_instances ].
+
+(* [fail_if_goal_contains_eval'] fails if the goal contains an occurrence
+   of [eval']. It does nothing otherwise. *)
+
+Ltac fail_if_goal_contains_eval' :=
+  lazymatch goal with |- context[eval'] => fail | _ => idtac end.
+
+(* [simp_eval] rewrites [eval] to [eval'], then reduces the goal, hopefully
+   expanding [eval'] away. It checks that [eval'] has indeed been
+   eliminated, and fails otherwise. *)
+
+Ltac simp_eval :=
+  simple eapply advance_simp_eval;
+  cbn -[app]; (* TODO or: [simpl eval']? *)
+    (* TODO decide how much reduction must be done here, and how *)
+  fail_if_goal_contains_eval'.
+    (* TODO The goal could still contain [eval'] at this point if [eval']
+       is applied to an opaque expression. There is currently an example
+       of this in records_proof.v, where we do caller-side reasoning.
+       We may abandon this style in the future. This expensive test
+       could then become unnecessary. *)
+
+(* The tactics [simp0] and [simp1] expect a goal of the form [simp m1 m2].
+
+   They advance this goal by performing simplification steps that lead from
+   [m1] to [m'1] and by leaving a residual goal of the form [simp m'1 m2].
+
+   Whereas [simp0] may find zero or more simplification steps, [simp1] must
+   find at least one simplification step; otherwise, it fails.
+
+   The term [m1] has *not* necessarily been reduced (by [cbn], [simpl] or
+   other means). If the tactics find that [m1] can be reduced, then they
+   do so, and they are careful to perform reduction only where necessary:
+   e.g. in the left-hand side of a [bind] but not in its right-hand side.
+
+   In some cases, the tactics are allowed to solve the goal. Of course this
+   must be done only in situations where we are certain (or have reasonable
+   grounds to believe) that the term has been simplified as far as possible
+   and cannot be further simplified. *)
+Ltac simp0 :=
+  (* We are allowed to perform zero or more steps. *)
+  (* Either perform at least one step, or perform zero step. *)
+  first [
+      eapply advance_simp_let; [ simp0 | ]
+    | eapply advance_simp_letrec; [ reflexivity | ]
+    | eapply advance_simp_mexpr; simp0
+    | eapply advance_simp_ilet; [simp0 | ]
+    | eapply advance_simp_iletrec; [ reflexivity | ]
+    | eapply advance_simp_imodule; [ simp0 | ]
+    | try simp1
+    ]
+
+with simp1 :=
+  (* We must perform at least one step. *)
+  (* We do not invoke Coq's reduction tactics ([cbn], [simpl], etc.) up front
+     because they are not selective; they perform reduction everywhere in the
+     goal. Instead, we first try to apply one of the following rewriting rules
+     at the root of the goal: *)
+  first [
+    (* Exploit an assumption, if we have one. *)
+    eassumption
+    (* Transform [try] into [bind]. *)
+  | simple eapply advance_simp_bind_as_try; simp0
+    (* Perform tail call optimisation. (Not essential.) *)
+  |  simple eapply advance_simp_bind_ret_right; simp0
+    (* Hoist left-nested [bind]s and [try]s. *)
+  | simple eapply advance_simp_bind_bind; simp0
+  | simple eapply advance_simp_bind_try; simp0
+  | simple eapply advance_simp_try_bind; simp0
+  | simple eapply advance_simp_try_try; simp0
+    (* Handle [Stop] effects. *)
+  | simple eapply advance_SimpEvalRetThrow'; simp0
+  | simple eapply advance_SimpEvalRetThrow; simp0
+  | simple eapply advance_SimpEvalThrow; simp0
+  | simple eapply advance_SimpEval; simp0
+      (*| simple eapply advance_SimpLoopThrow; simp0 *)
+      (*| simple eapply advance_SimpLoop; simp0 *)
+  | simple eapply advance_SimpEvalEAssert; simp0
+      (* We do not deal with [choose] in its full generality. Instead,
+         we provide ad hoc support for [EAssert] expressions, which
+         currently are the only place where [choose] is used. *)
+    (* Handle [val_as_bool], which is opaque. *)
+  | simple eapply advance_simp_val_as_bool_VTrue; simp0
+  | simple eapply advance_simp_val_as_bool_VFalse; simp0
+  | simple eapply advance_simp_val_as_bool_VBool; simp0
+
+  | simple eapply advance_simp_is_module_val_as_struct; done
+  | simple eapply advance_simp_is_module_lookup_name;
+    [ done | by eauto using in_eq, in_cons ]
+
+  | simple eapply advance_simp_pure_spec_val_as_struct; done
+  | simple eapply advance_simp_pure_spec_lookup_name;
+    [ done | by eauto using in_eq, in_cons ]
+
+  (* TODO the following 4 rules are useful only in pre/postconditions,
+     not in [simp] goals *)
+  (*
+  | rewrite -> Zeq_spec; simp0 (* x =? y ↔ x = y *)
+  | rewrite -> Zne_spec; simp0 (* negb (x =? y) ↔ x ≠ y *)
+  | rewrite -> Zlt_spec; simp0 (* x <? y ↔ x < y *)
+  | rewrite -> Zle_spec; simp0 (* negb (y <? x) ↔ x ≤ y *)
+   *)
+    (* If none of the above rules can be applied, then we inspect the syntax
+       of the goal and, based on it, we try to do something smart. *)
+  | simp1_inspect
+    (* As a last resort, if none of the above cases fire, it may be the case
+       that we are facing a term that needs to be reduced by Coq. This could
+       be, for instance, a pair deconstruction [let '(a, b) := t1 in t2], or
+       an application of one the interpreter's auxiliary functions. We
+       perform this reduction step only if it is nontrivial. *)
+    (* One might wish to perform this reduction step only if it is nontrivial
+       AND it enables at least one further simplification step. That would be
+       expressed by using [simp1] instead of [simp0] below. However, that
+       would be too restrictive. Indeed, this reduction step can lead us to a
+       situation where a breakpoint is visible and no further simplification
+       is possible. *)
+    (* TODO is this a good idea? could this be very expensive? *)
+  | progress normalize; simp0
+  ]
+
+(* Like [simp1], [simp1_inspect] expects a goal of the form [simp m1 _],
+   and additionally expects that the term [m1] cannot be rewritten using
+   any of the rewriting rules listed above. *)
+
+with simp1_inspect :=
+  (* Examine the syntax of [m1]. *)
+  (* Note that we do *not* reduce [m1] before inspecting it. *)
+  lazymatch goal with |- simp ?m1 _ =>
+  lazymatch m1 with
+  | ret ?a1 =>
+      fail
+  | lookup_name ?η ?x =>
+      (* We may be able to prove [lookup_name η x = ret v], for some [v],
+         either simply by reducing this lookup, or by exploiting a hypothesis
+         or a hint database. *)
+      simple eapply simp_reflexive_ret; [
+        (* subgoal: [m1 = ret v] *)
+        solve [ eauto with simp_specs ]
+      ]
+  | eval ?η ?e =>
+      first [
+        (* Attempt 1. Solve the goal by exploiting the hint database
+           [simp_specs]. This can be necessary if the user chooses to
+           populate the hint database with specifications about terms
+           of the form [eval η e], as opposed to [call v1 v2]. *)
+        simp_solve_eauto
+      |
+        (* Attempt 2. Unfold the definition of [eval] once in [eval η e]. *)
+        simp_eval; simp0
+      ]
+  | call ?v1 ?v2 =>
+      first [
+        (* Attempt 1. Step into the call. This is possible only if [v1]
+           is a concrete closure. *)
+        simp_enter; simp0
+        (* Attempt 2. Reason about this call. This is possible only if a
+           specification for this call exists in the current context or
+           in a hint database. *)
+      | simp1_call_reason v2
+      ]
+  | bind ?m ?f =>
+      (* We want to first simplify the left-hand side of [bind], as far as
+         possible; then, if possible, simplify the [bind] combinator away
+         and further simplify the result. Two attempts are needed to ensure
+         that we make one step of progress in at least one of the two
+         subgoals. This should nevertheless be reasonably efficient. *)
+      first [
+        (* Attempt 1. Make progress on the left-hand side,
+           and possibly more progress thereafter. *)
+        simple eapply advance_SimpBind; [ simp1; simp_close | simp0_bind ]
+      |
+        (* Attempt 2. Make progress by eliminating this [bind],
+           and possibly more progress thereafter. *)
+        simp1_bind
+      ]
+  | try ?m ?f ?h =>
+      (* [try] is treated in the same way as [bind]. *)
+      first [
+        simple eapply advance_SimpTry; [ simp1; simp_close | simp0_try ]
+      | simp1_try
+      ]
+  | Par ?m1l ?m1r ?k ?h =>
+      (* We want to first simplify both sides of the [Par] independently, as
+         far as possible; then, if possible, simplify the [Par] combinator
+         away and further simplify the result. Three attempts are needed to
+         ensure that we make one step of progress in at least one of the
+         three subgoals. This should nevertheless be reasonably efficient. *)
+      first [
+        (* Attempt 1. Make progress on the left-hand side,
+           and possibly more progress elsewhere. *)
+        simple eapply advance_SimpPar; [ simp1; simp_close | simp0; simp_close | simp0_par ]
+      |
+        (* Attempt 2. Make progress on the right-hand side,
+           and possibly more progress elsewhere. *)
+        simple eapply advance_SimpPar; [ simp_close | simp1; simp_close | simp0_par ]
+      |
+        (* Attempt 3. Make progress by eliminating this [Par],
+           and possibly more progress thereafter. *)
+        simp1_par
+      ]
+  end end
+
+(* [simp_enter] expects a goal of the form [simp (call _ _) _] and steps
+   into the call (if possible). It leaves one subgoal. *)
+
+with simp_enter :=
+  (* We intentionally use [eapply], not [simple eapply], so that [v1] can be
+     unfolded on the fly if necessary. This is useful, e.g., when [v1] is a
+     function in the standard library, such as [Stdlib__not].
+
+     We expect [eapply] to succeed only if [v1] is a concrete closure, that
+     is, either [VClo ...] or [VCloRec ...] or a transparent definition that
+     unfolds to one of these forms. If [v1] is an opaque definition then we
+     expect [eapply] to fail. (These expectations may be wrong. I have
+     observed situations where [eapply] violates opacity.) *)
+  first [
+    (* strong *) eapply simp_enter_call_VClo
+  | (* strong *) eapply simp_enter_call_VCloRec
+  ]
+
+(* [simp_call] expects a goal of the form [simp (call _ _) _] and solves
+   this goal using a specification that must exist in the current context or
+   in the hint database [simp_specs].
+
+   This tactic leaves zero subgoals. If the goal cannot be solved, then
+   this tactic fails. *)
+
+with simp1_call_reason v2 :=
+  lazymatch v2 with
+  | #(?x2) =>
+      (* The actual argument is already encoded. Fine. *)
+      (* We reason about function calls using whatever hypotheses may be
+         present in the context and in the hint database [simp_specs]. *)
+      simp_solve_eauto
+  | _ =>
+      (* The actual argument is not yet encoded. It may or may not be
+         necessary to encode it, depending on the specification on the
+         function that is called. *)
+      first [
+        simp_solve_eauto
+      | simple eapply simp_call; [ solve [ encode ] | simp_solve_eauto ]
+      ]
+  end
+
+(* [simp0_bind] and [simp1_bind] are special cases of [simp0] and [simp1].
+
+   They assume that the goal is of the form [simp (bind m _) _],
+   where [m] has been simplified already. *)
+
+with simp0_bind :=
+  try simp1_bind
+
+with simp1_bind :=
+  (* Performing at least one simplification step, when the term is a [bind]
+     construct, requires rewriting [bind (ret _) _]. To do so, we explicitly
+     apply a lemma; this ensures that we fail if the goal is not of the form
+     [bind (ret _) _]. *)
+  (* TODO explain that we wish to allow [m] to reduce to [ret _],
+          without violating opacity *)
+  first [
+    simple eapply advance_simp_bind_ret
+  | lazymatch goal with
+    |- simp (bind ?m _) _ =>
+      let o := eval cbn -[app] in m in
+      lazymatch o with ret _ =>
+        (* strong *) eapply advance_simp_bind_ret
       end
+    end
+  ];
+  simp0
+
+(* [simp0_try] and [simp1_try] are special cases of [simp0] and [simp1].
+
+   They assume that the goal is of the form [simp (try m _ _) _],
+   where [m] has been simplified already. *)
+
+with simp0_try :=
+  try simp1_try
+
+with simp1_try :=
+  (* TODO we cut corners and use strong [eapply] here; this is simpler;
+          we need not worry about opacity because breakpoints do not
+          appear under [try] *)
+  first [
+    (* strong *) eapply advance_simp_try_ret
+  | (* strong *) eapply advance_simp_try_throw
+  ];
+  simp0
+
+(* [simp0_par] and [simp1_par] are special cases of [simp0] and [simp1].
+
+   They assume that the goal is of the form [simp (Par m1 m2 _ _) _],
+   where [m1] and [m2] have been simplified already. *)
+
+with simp0_par :=
+  try simp1_par
+
+with simp1_par :=
+  (* Performing at least one simplification step, when the term is a [Par]
+     construct, requires applying one of the following rules. *)
+  (* TODO we cut corners and use strong [eapply] here; this is simpler;
+          we need not worry about opacity because breakpoints do not
+          appear under [par] *)
+  first [
+    (* strong *) eapply advance_SimpParRetRet (* maybe a special case of the following *)
+  | (* strong *) eapply advance_SimpParRetLeftThrow
+  | (* strong *) eapply advance_SimpParRetLeft
+  | (* strong *) eapply advance_SimpParRetRightThrow
+  | (* strong *) eapply advance_SimpParRetRight
+  ];
+  simp0.
+
+(* [simp] is the main public entry point into the above tactics. *)
+
+(* [simp] proves or advances a goal of the form [simp m1 m2], where [m2] may
+   be a metavariable. If [m2] is a metavariable then it is instantiated with
+   a term that has been simplified as far as possible. *)
+
+Ltac simp :=
+  lazymatch goal with
+  | |- simp ?m1 _ =>
+      simp0; try simp_close
+  | _ =>
+      fail "[simp] expects a goal of the form [simp _ _]"
   end.
 
-(* It is debatable in which order the two premises of the lemma [pure_call]
-   should be attacked. The premise [v'2 = #x] may seem easy to solve (this
-   is the job of the tactic [encode]) so one may wish to solve it first.
-   This offers the advantage of instantiating [x] immediately, so [x] is
-   known when we try to prove that the call is permitted -- which may
-   involve proving that a precondition holds.
+(* [simp_really] is another public entry point into the above tactics. *)
 
-   However, solving [v'2 = #x] can involve guessing some types (e.g., the
-   type of an empty list), and we have used [Hint Mode] in encode.v to
-   forbid this. So, it can also be preferable to first solve the premise
-   [pure (call v1 #x) φ]. Doing so can allow us to instantiate these types
-   in a correct way.
+(* [simp_really] proves a goal of the form [simp m1 m2], where [m2] must be
+   a metavariable. [m2] is instantiated with a term that has been simplified
+   as far as possible. [simp_really] performs at least one step of
+   simplification. *)
 
-   One might wish to try both approaches in sequence, but waiting until
-   [encode] fails is very slow (several seconds).
+Ltac simp_really :=
+  lazymatch goal with |- simp ?m1 _ =>
+    simp1; simp_close
+  | _ =>
+    fail "[simp_really] expects a goal of the form [simp _ _]"
+  end.
 
-   One might also wish to do a bit of both: that is, first apply some lemma
-   [L] to the subgoal [pure (call v1 #x) φ], then solve [v'2 = #x], then
-   attack the proof obligations created by applying the lemma [L]. *)
+(* [simp_enter_and_abstract] expects a goal of the form [simp (call v _) _],
+   where [v] is a concrete closure (typically a recursive closure). It steps
+   into the call, then abstracts away the closure [v], so as to make it
+   opaque. *)
 
-Create HintDb pure_specs.
-
-(* TODO may be unused *)
-Ltac pure_call :=
-  first [
-    simple eapply pure_call; [ solve [encode] | solve [eauto with pure_specs] ]
-  | simple eapply pure_consequence; [
-      simple eapply pure_call; [ solve [encode] | eauto with pure_specs ]
-    | cbn ]
-  ].
-
-Ltac pure_enter_and_abstract :=
-  lazymatch goal with |- pure (call ?v _) _ =>
+Ltac simp_enter_and_abstract :=
+  lazymatch goal with |- simp (call ?v _) _ =>
     (* First, expand [call] away. *)
-    pure1_call_step;
+    simp_enter;
     normalize;
     (* Second, abstract away the closure (of which there are typically
        several occurrences in the hypotheses and goal), replacing it
@@ -279,225 +928,26 @@ Ltac pure_enter_and_abstract :=
 
 (* -------------------------------------------------------------------------- *)
 
-(* Evaluate an [eval] by repeatedly changing [eval] into [eval'] *)
-Ltac simp_evaluate :=
-  simpl; repeat (rewrite eval_eval'; simpl).
+(* The tactic [simp_specify x φ] should be used when the term begins with
+   [bind (ret_concat δ η) _], that is, when the environment is about to be
+   extended with the environment fragment [δ].
 
-(* TODO the following tactics seem redundant with the symbolic execution
-        tactics, [simp] and friends. Avoid duplication. *)
+   The tactic looks up the variable [x] in the environment fragment [δ]
+   so as to find the value [v] of this variable. Then, it produces two
+   subgoals:
+   - the subgoal [φ v],
+     letting the user prove that [v] satisfies the specification [φ];
+   - the original goal,
+     generalized under the form [∀ v, φ v → ...],
+     which means that [v] becomes an opaque value
+     about which nothing is known except that [φ v] holds. *)
 
-(* On a goal of the form [pure (Stop CEval x k ko) φ], evaluate the call by:
-   stepping through the [Stop] with the appropriate advance_SimpEval lemma,
-   using [simp_evaluate] under the resulting pure *)
-Ltac pure_evaluate :=
-  (lazymatch goal with
-   | |- pure (Stop CEval _ _ _) _ =>
-       eapply pure_simp; [
-         first [
-           apply advance_SimpEvalRetThrow
-         | apply advance_SimpEvalThrow
-         | apply advance_SimpEval
-         ]
-       | apply SimpReflexive
-       ]
-   | _ => idtac
-   end);
-  eapply pure_simp; [simp_evaluate; apply SimpReflexive|].
-
-Ltac SimpParRet :=
-  first [
-    apply SimpParRetRet
-  | apply SimpParRetLeftThrow
-  | apply SimpParRetRightThrow
-  | apply SimpParRetLeft
-  | apply SimpParRetRight
-  ].
-
-Ltac pureParRet :=
-  eapply pure_simp; first SimpParRet; simpl.
-
-(* -------------------------------------------------------------------------- *)
-
-(* Dummy proposition with one constructor *)
-Inductive BLOCK := block.
-
-(* Tranform a goal of the form [H1 -> H2 -> ... -> BLOCK -> G] into
-   [H1 /\ H2 /\ ... -> G] *)
-Ltac conj_until_BLOCK b :=
+Ltac simp_specify x φ :=
   lazymatch goal with
-  | |- BLOCK -> _ =>
-      intros _; let H := fresh in
-               pose proof (H := I); revert H
-  | |- _ -> BLOCK -> _ =>
-      let H1 := fresh in
-      intros H1 _; revert H1
-  | |- ?A -> ?B -> _ =>
-      let H1 := fresh in
-      let H2 := fresh in
-      let H3 := fresh in
-      intros H1 H2; pose proof (H3 := conj H2 H1);
-      revert H3;
-      match b with
-      | true => clear H1; conj_until_BLOCK true
-      | false => conj_until_BLOCK true
+    |- simp (eval (?δ ++ _) _) _ =>
+      let o := eval cbn in (lookup_name δ x) in
+      lazymatch o with ret ?v =>
+        let h := fresh in
+        assert (φ v) as h; [| revert h; generalize v ]
       end
   end.
-
-(* Given a tuple (or single term), move all hypotheses depending on elements
-   of the tuple (or single term) into the goal *)
-Ltac generalize_tuple t :=
-  match t with
-  | pair ?x ?y =>
-      generalize dependent y; intro;
-      generalize_tuple x
-  | _ => generalize dependent t; intro
-  end.
-
-(* Given a term (or tuple of terms), move all hypotheses depending on this term
-   (or tuple of terms) into the goal as a single conjunction *)
-Ltac capture_hypotheses_aux arg :=
-  generalize (block);
-  generalize_tuple arg;
-  conj_until_BLOCK false.
-
-Tactic Notation "capture_hypotheses" constr(arg1) :=
-  capture_hypotheses_aux arg1.
-
-Tactic Notation "capture_hypotheses" constr(arg1) "as" simple_intropattern(x) :=
-  capture_hypotheses_aux arg1; intros x.
-
-Tactic Notation "capture_hypotheses" constr(arg1) constr(arg2) :=
-  capture_hypotheses_aux (arg1, arg2).
-
-Tactic Notation "capture_hypotheses" constr(arg1) constr(arg2) "as" simple_intropattern(x) :=
-  capture_hypotheses_aux (arg1, arg2); intros x.
-
-(* Automatically apply [pure_rec_call] on a goal of the form [pure m φ] *)
-Ltac pure_rec_tac arg pre Hwf :=
-  (* Eta-expand the postcondition *)
-  match goal with
-  | |- pure _ ?H =>
-      let post := fresh in
-      set (post := H); pattern arg in post; cbv delta [post]; clear post
-  end;
-  (* Apply [pure_rec_call], possibly with an explicit precondition *)
-  match pre with
-  | None =>
-      eapply pure_rec_call with (v:=arg)
-  | Some ?pre =>
-      eapply pure_rec_call with (v:=arg) (P:=pre)
-  end;
-  (* Try and solve subgoals generated by [pure_rec_call] *)
-  [ apply Hwf
-  | lazymatch pre with
-    | None =>
-        capture_hypotheses arg;
-        let HPre := fresh in intros HPre;
-        pattern arg in HPre;
-        exact HPre
-    | Some _ =>
-        subst; auto; fail
-    end
-  | ];
-  clear dependent arg; (* [pure_rec_call] deprecates the original argument *)
-  let HP := fresh "HP" in
-  let IH := fresh "IH" in
-  simpl; intros vf arg HP IH.
-
-Tactic Notation "pure_rec" constr(arg) constr(Hwf) :=
-  pure_rec_tac arg constr:(@None False) Hwf.
-
-Tactic Notation "pure_rec" constr(arg) constr(pre) constr(Hwf) :=
-  pure_rec_tac arg constr:(Some pre) Hwf.
-
-(* Automatically apply [pure_nested_call] on a goal of the form [pure m φ] *)
-Ltac pure_nested_tac arg1 arg2 pre Hwf :=
-  match goal with
-  | |- pure _ (fun c => pure _ ?H) =>
-      let post := fresh in
-      set (post := H); pattern arg1, arg2 in post; cbv delta [post]; clear post;
-      lazymatch pre with
-      | None =>
-          eapply pure_nested_call with (v1:=arg1) (v2:=arg2)
-      | Some ?pre =>
-          eapply pure_nested_call with (v1:=arg1) (v2:=arg2) (P:=pre)
-      end;
-      [ reflexivity
-      | simpl; rewrite eval_eval'; reflexivity
-      | apply Hwf
-      | lazymatch pre with
-          None =>
-            capture_hypotheses arg1 arg2;
-            let HPre := fresh in intros HPre;
-                                 pattern arg1, arg2 in HPre;
-                                 exact HPre
-        | Some _ =>
-            auto
-        end
-      | ];
-      let HP := fresh "HP" in
-      let IH := fresh "IH" in
-      clear dependent arg1 arg2;
-      simpl; intros vf arg1 arg2 HP IH
-  end.
-
-Tactic Notation "pure_nested" constr(arg1) constr(arg2) constr(Hwf) :=
-  pure_nested_tac arg1 arg2 constr:(@None False) Hwf.
-
-Tactic Notation "pure_nested" constr(arg1) constr(arg2)
-  constr(pre) constr(Hwf) :=
-  pure_nested_tac arg1 arg2 constr:(Some pre) Hwf.
-
-(* -------------------------------------------------------------------------- *)
-
-Module Tac.
-  Import Ltac2.
-
-  Ltac2 eta_post' (arg : constr list) :=
-    lazy_match! goal with
-    | [ |- pure _ ?φ ] =>
-        let post := Fresh.in_goal @post in
-        set ($post := $φ);
-        Std.pattern (List.map (fun x => (x, Std.AllOccurrences)) arg)
-          { Std.on_hyps := Some [(post, Std.AllOccurrences, Std.InHyp)];
-                           Std.on_concl := Std.NoOccurrences };
-        cbv delta [&post];
-        clear $post
-    end.
-
-  Import Constr.Unsafe.
-
-  Ltac2 eta_post'' (arg : Ltac1.t) :=
-    let arg := Option.get (Ltac1.to_list arg) in
-    let arg := List.map (fun x => Option.get (Ltac1.to_constr x)) arg in
-    eta_post' arg.
-
-  Ltac eta_post arg :=
-    let f := ltac2:(arg |- eta_post'' arg) in
-    f arg.
-
-  Tactic Notation "eta_post" constr_list(arg) :=
-    let f := ltac2:(arg |- eta_post'' arg) in
-    f arg.
-
-  Ltac2 eta_tuple_aux t :=
-    let rec aux t :=
-      lazy_match! t with
-      | pair ?x ?y =>
-          let l := aux x in
-          List.append l [y]
-      | ?single => [single]
-      end
-    in
-    let arg_list := aux t in
-    eta_post' arg_list.
-
-  Ltac2 eta_tuple_aux_interface (arg : Ltac1.t) :=
-    let arg := Option.get (Ltac1.to_constr arg) in
-    eta_tuple_aux arg.
-
-  Tactic Notation "eta_tuple" constr(arg) :=
-    let f := ltac2:(arg |- eta_tuple_aux_interface arg) in
-    f arg.
-
-End Tac.
