misc/attic/specification_tactics.v
@@ -1,0 +1,146 @@
+From osiris Require Import osiris.
+From osiris.stdlib Require Import Stdlib.
+From osiris.examples Require Import og_splay.
+
+(* -------------------------------------------------------------------------- *)
+(* Specification structures. *)
+
+(* Given a name which corresponds to the declaration, there is some pspec *)
+Class decl_spec (name : var) := { Decl_spec : pspec }.
+
+(* Smart constructor *)
+Definition val_spec (name : var) `{decl_spec name} (v : val) : Prop :=
+  @Decl_spec name _ v.
+
+(* Lifting specification over declaration to a specification over an environment:
+    i.e. the declaration can be found the environment and satisfies the
+    specification. *)
+Definition spec (name : var) `{decl_spec name} (η : env) : Prop :=
+  let val_spec := @Decl_spec name _ in
+  pure (lookup_name η name) val_spec.
+
+(* -------------------------------------------------------------------------- *)
+(* Specification of [splay]. *)
+
+(* Names for the functions we would like to specify *)
+Definition SPLAY := "splay".
+Definition SPLAY_LEAF := "splay_leaf".
+Definition ZLOOKUP := "zlookup".
+
+(* Specification for each function *)
+Definition splay_spec :=
+  fun splay =>
+    ∀ A `(_ : Encode A) (ctx : zipper A) (l : tree A) (x : A) (r : tree A),
+    pure
+      (call splay #(l, x, r, ctx))
+      (λ t', fringe t' = fringe (fill ctx (Node l x r))).
+
+Definition splay_leaf_spec :=
+  fun (splay_leaf : val) =>
+    ∀ A `(_ : Encode A) (ctx : zipper A),
+    pure
+      (call splay_leaf #ctx)
+      (λ t', fringe t' = fringe (fill ctx Leaf)).
+
+Definition zlookup_spec :=
+  fun (zlookup : val) =>
+    ∀ A `(_ : Encode A) (le : A → A → Prop) `(_ : PreOrder _ le),
+      compare_spec Stdlib__compare le →
+      ∀ (t : tree A) (x : A) (ctx : zipper A),
+      bst (strict le) t →
+      pure
+        (call zlookup #(t, x, ctx))
+        (λ '(oy, t'),
+          member le x (fringe t) oy ∧
+          fringe t' = fringe (fill ctx t)).
+
+#[local] Instance splay_decl_spec : decl_spec SPLAY :=
+  {| Decl_spec := splay_spec |}.
+
+#[local] Instance splay_leaf_decl_spec : decl_spec SPLAY_LEAF :=
+  {| Decl_spec := splay_leaf_spec |}.
+
+#[local] Instance zlookup_decl_spec : decl_spec ZLOOKUP :=
+  {| Decl_spec := zlookup_spec |}.
+
+(* -------------------------------------------------------------------------- *)
+
+(* Top-level environment of [splay]. *)
+
+Definition stdlib_env := ("Stdlib", Stdlib) :: Stdlib_env.
+
+(* Ltac programming to compute the environment from [mexpr]'s. *)
+
+(* Instantiates an evar and tries to apply the aggressive [simp_really] resolution
+   spitting out a [micro] monad if it succeeds. *)
+Ltac try_reduce_with_simp A E m :=
+  let e := fresh "e" in
+  let H := fresh "H" in
+  evar (e : micro A E);
+  assert (H:simp m ?e) by simp_really;
+  clear H;
+  exact e.
+
+(* Given a module definition that has been evaluated, return the environment that
+ is built from the evaluated module. *)
+Ltac extract_env module_def :=
+  let m := fresh "m" in
+  let l := fresh "l" in
+  pose module_def as m;
+  unfold module_def in m;
+  match goal with
+  | m := ret (VStruct ?x) |- _ => pose x as l
+  end; clear m; cbn in *; exact l.
+
+(* We can extract the environment programmatically. *)
+Definition splay_module_env' :=
+  (ltac:(with_strategy transparent [eval_bindings eval_mexpr extend] try_reduce_with_simp val void (eval_mexpr stdlib_env __main))).
+(* A more sane approach would be to state some well-formedness conditions *)
+
+(* Extracted environment *)
+Definition splay_module_env : env :=
+  ltac:(extract_env splay_module_env').
+
+(* -------------------------------------------------------------------------- *)
+
+(* Util functions for specs *)
+Ltac start_proof := unfold spec; cbn; pure1; red.
+
+(* If a specification holds for an environment, we know that there exists some
+   declaration in the environment that satisfies the specification. *)
+(* TODO fp: It seems to me that this lemma goes too far.
+        It essentially expands away the judgement
+        [pure (lookup_name η name) val_spec]
+        but we should we able to exploit this judgement
+        without expanding it. *)
+Lemma invert_spec :
+  forall x `{decl_spec x} env,
+    spec x env ->
+    ∃ v, lookup_name env x = ret v /\ val_spec x v.
+Proof.
+  intros x Spec env; revert x Spec.
+  induction env.
+  intros * Hspec. red in Hspec; cbn in Hspec.
+  - unfold lookup_name in Hspec.
+    destruct Hspec as (?&Hspec&?).
+    with_strategy transparent [missing_variable_or_field]
+      unfold missing_variable_or_field in Hspec.
+    clarify_simp.
+  - intros * Hspec. red in Hspec.
+    unfold lookup_name in *. destruct a.
+    destruct (x =? v)%string.
+    + destruct Hspec as (?&?&Hspec). clarify_simp.
+      eexists; split; eauto.
+    + fold lookup_name in *. eapply IHenv; eauto.
+Qed.
+
+(* Apply the specification of a function *)
+Ltac apply_spec SPEC :=
+  let H := fresh "H" in
+  let vspec := fresh "vspec" in
+  let Hlu := fresh "Hlu" in
+  pose proof (invert_spec _ _ SPEC) as H;
+  destruct H as (?&Hlu&vspec);
+  inversion Hlu; subst;
+  try solve [eapply vspec];
+  try (eapply pure_consequence ; first eapply vspec).
